Add crypto implementation

fstar/new/Crypto.fsti
@@ -1,5 +1,50 @@
 module Crypto
 
+open Lib.Result
+
+open Spec.Agile.DH
+open Spec.Agile.AEAD
+open Spec.Agile.Hash
+open Lib.RandomSequence
+
+module DH = Spec.Agile.DH
+module AEAD = Spec.Agile.AEAD
+module Hash = Spec.Agile.Hash
+module Rand = Lib.RandomSequence
+
+(*** Ciphersuite ***)
+
+val ciphersuite: Type0
+
+(*** KDF ***)
+
+val kdf_length: ciphersuite -> nat
+
+val kdf_extract_tot: cs:ciphersuite -> key:bytes{Seq.length key < pow2 31} -> data:bytes{Seq.length data < pow2 60} -> lbytes (kdf_length cs)
+val kdf_expand_tot: cs:ciphersuite -> prk:bytes{kdf_length cs <= Seq.length prk /\ Seq.length prk <= pow2 31} -> info:bytes{Seq.length info <= pow2 60} -> len:nat{len <= 4080} -> lbytes len
+
+val kdf_extract: cs:ciphersuite -> key:bytes -> data:bytes -> result (lbytes (kdf_length cs))
+val kdf_expand: cs:ciphersuite -> prk:bytes -> info:bytes -> len:nat -> result (lbytes len)
+
+(*** HPKE ***)
+
+val hpke_public_key_length: ciphersuite -> nat
+val hpke_private_key_length: ciphersuite -> nat
+val hpke_kem_output_length: ciphersuite -> nat
+
+type hpke_public_key (cs:ciphersuite) = lbytes (hpke_public_key_length cs)
+type hpke_private_key (cs:ciphersuite) = lbytes (hpke_private_key_length cs)
+type hpke_kem_output (cs:ciphersuite) = lbytes (hpke_kem_output_length cs)
+
+val hpke_encrypt: cs:ciphersuite -> Rand.entropy -> pkR:hpke_public_key cs -> info:bytes -> ad:bytes -> plaintext:bytes -> Rand.entropy & result (hpke_kem_output cs & bytes)
+val hpke_decrypt: cs:ciphersuite -> enc:hpke_kem_output cs -> skR:hpke_private_key cs -> info:bytes -> ad:bytes -> ciphertext:bytes -> result bytes
+
+(*** String to bytes ***)
+
+let string_is_ascii (s:string) = List.Tot.for_all (fun x -> FStar.Char.int_of_char x < 256) (FStar.String.list_of_string s)
+val string_to_bytes: s:string{b2t (normalize_term (string_is_ascii s))} -> lbytes (String.strlen s)
+
+(*
 open FStar.Mul
 open Lib.IntTypes
 open Lib.Sequence
@@ -60,3 +105,5 @@ val unpad: bytes_t -> result bytes_t
 val hash: bytes_t -> result bytes_t
 val mac: bytes_t -> bytes_t -> result bytes_t
 val mac_verify: bytes_t -> bytes_t -> bytes_t -> bool
+
+*)
