fstar/new/Crypto.fst
@@ -1,0 +1,143 @@
+module Crypto
+
+open Lib.Sequence
+open Lib.ByteSequence
+open Lib.IntTypes
+
+open Spec.Agile.HKDF
+open FStar.Mul
+open Spec.Hash.Definitions
+
+open Spec.Agile.DH
+open Spec.Agile.AEAD
+open Spec.Agile.Hash
+open Spec.Agile.HKDF
+open HPKE
+
+module DH = Spec.Agile.DH
+module AEAD = Spec.Agile.AEAD
+module Hash = Spec.Agile.Hash
+module HKDF = Spec.Agile.HKDF
+module HPKE = HPKE
+
+(*** Ciphersuite ***)
+
+type ciphersuite_t = {
+  kem_dh:  DH.algorithm;
+  kem_hash: Hash.algorithm;
+  aead: AEAD.alg;
+  kdf_hash: Hash.algorithm;
+  //TODO: signature
+}
+
+val is_valid_ciphersuite_t: ciphersuite_t -> bool
+let is_valid_ciphersuite_t cs =
+  HPKE.is_valid_hash (cs.kem_hash) &&
+  HPKE.is_valid_kem (cs.kem_dh, cs.kem_hash) &&
+  HPKE.is_valid_aead (HPKE.Seal cs.aead) &&
+  HPKE.is_valid_hash (cs.kdf_hash)
+
+let ciphersuite = cs:ciphersuite_t{is_valid_ciphersuite_t cs}
+
+val ciphersuite_to_hpke_ciphersuite: ciphersuite -> HPKE.ciphersuite
+let ciphersuite_to_hpke_ciphersuite cs =
+  (cs.kem_dh, cs.kem_hash, HPKE.Seal cs.aead, cs.kdf_hash)
+
+(*** KDF ***)
+
+val max_input_length_bound: a:Hash.hash_alg -> Lemma (pow2 61 - 1 <= max_input_length a)
+let max_input_length_bound a =
+  FStar.Math.Lemmas.pow2_le_compat 128 61;
+  FStar.Math.Lemmas.pow2_le_compat 125 61;
+  FStar.Math.Lemmas.pow2_le_compat 64 61
+
+let kdf_length cs = hash_length cs.kdf_hash
+
+let kdf_extract_tot cs key data =
+  assert (block_length (cs.kdf_hash) <= 128);
+  max_input_length_bound (cs.kdf_hash);
+  assert_norm (pow2 60 < pow2 61 - 129); //==> Seq.length data + block_length a <= max_input_length a
+  assert_norm (pow2 31 < pow2 32 - 128); //==> keysized (Seq.length key)
+  assert_norm (pow2 31 < pow2 61 - 1); //==> keysized (Seq.length key)
+  extract (cs.kdf_hash) key data
+
+let kdf_expand_tot cs prk info len =
+  assert(16 <= hash_length cs.kdf_hash);
+  assert (hash_length cs.kdf_hash <= 64);
+  assert (block_length cs.kdf_hash <= 128);
+  max_input_length_bound cs.kdf_hash;
+  assert_norm(pow2 60 < pow2 61 - 194); //==> hash_length a + Seq.length info + 1 + block_length a <= max_input_length a
+  assert_norm(pow2 31 < pow2 32 - 128); //==> keysized (Seq.length prk)
+  assert_norm(pow2 31 < pow2 61 - 1); //==> keysized (Seq.length prk)
+  expand cs.kdf_hash prk info len
+
+let kdf_extract cs key data =
+  if not (Seq.length key <= max_input_length cs.kdf_hash && Seq.length key + block_length cs.kdf_hash < pow2 32) then
+    Error "kdf_extract_dyn: bad key size"
+  else if not (Seq.length data + block_length (cs.kdf_hash) <= max_input_length (cs.kdf_hash)) then
+    Error "kdf_extract_dyn: bad data size"
+  else
+    Success (extract (cs.kdf_hash) key data)
+
+let kdf_expand cs prk info len =
+  if not (hash_length cs.kdf_hash <= Seq.length prk) then
+    Error "kdf_expand_dyn: prk too small"
+  else if not (Seq.length prk <= max_input_length cs.kdf_hash && Seq.length prk + block_length cs.kdf_hash < pow2 32) then
+    Error "kdf_expand_dyn: prk too long"
+  else if not (hash_length cs.kdf_hash + Seq.length info + 1 + block_length cs.kdf_hash <= max_input_length cs.kdf_hash) then
+    Error "kdf_expand_dyn: info too long"
+  else if not (len <= 255 * hash_length cs.kdf_hash) then
+    Error "kdf_expand_dyn: len too high"
+  else
+    Success (expand cs.kdf_hash prk info len)
+
+(*** HPKE ***)
+
+let hpke_public_key_length cs = HPKE.size_dh_public (ciphersuite_to_hpke_ciphersuite cs)
+let hpke_private_key_length cs = HPKE.size_dh_key (ciphersuite_to_hpke_ciphersuite cs)
+let hpke_kem_output_length cs = HPKE.size_dh_public (ciphersuite_to_hpke_ciphersuite cs)
+
+let hpke_encrypt cs entropy pkR info ad plaintext =
+  let (new_entropy, random_bytes) = Rand.crypto_random entropy (hpke_private_key_length cs) in
+  match HPKE.derive_key_pair (ciphersuite_to_hpke_ciphersuite cs) random_bytes with
+  | None -> (new_entropy, Error "hpke_encrypt: HPKE.derive_key_pair failed")
+  | Some (skE, _) -> (
+    let pkR = HPKE.deserialize_public_key (ciphersuite_to_hpke_ciphersuite cs) pkR in
+    if not (Seq.length info <= max_length_info cs.kdf_hash) then
+      (new_entropy, Error "hpke_encrypt: info too long")
+    else if not (Seq.length ad <= AEAD.max_length cs.aead) then
+      (new_entropy, Error "hpke_encrypt: ad too long")
+    else if not (Seq.length plaintext <= AEAD.max_length cs.aead) then
+      (new_entropy, Error "hpke_encrypt: plaintext too long")
+    else (
+      match HPKE.sealBase (ciphersuite_to_hpke_ciphersuite cs) skE pkR info ad plaintext with
+      | None -> (new_entropy, Error "hpke_encrypt: HPKE.sealBase failed")
+      | Some (kem_output, ciphertext) -> (new_entropy, Success (kem_output, ciphertext))
+    )
+  )
+
+let hpke_decrypt cs enc skR info ad ciphertext =
+  if not (Seq.length info <= max_length_info cs.kdf_hash) then
+    Error "hpke_decrypt: info too long"
+  else if not (Seq.length ad <= AEAD.max_length cs.aead) then
+    Error "hpke_decrypt: ad too long"
+  else if not (Seq.length ciphertext >= AEAD.tag_length cs.aead) then
+    Error "hpke_decrypt: plaintext too short"
+  else (
+    match HPKE.openBase (ciphersuite_to_hpke_ciphersuite cs) enc skR info ad ciphertext with
+    | None -> Error "hpke_decrypt: HPKE.openBase failed"
+    | Some res -> Success res
+  )
+
+(*** String to bytes ***)
+
+let string_to_bytes s =
+  let open FStar.String in
+  let open FStar.Char in
+  let open FStar.List.Tot in
+  let rec aux (l:list char{for_all (fun x -> int_of_char x < 256) l}): lbytes (length l) =
+    match l with
+    | [] -> bytes_empty
+    | h::t -> FStar.Seq.append (create 1 (u8 (int_of_char h))) (aux t)
+  in
+  aux (list_of_string s)
